progress.v
@@ -10,6 +10,7 @@ Require Import reductions.
 Require Import typing.
 Require Import namesAndTypes.
 Require Import progress_sf.
+Require Import ocap.
 
 Require Import wf_env.
 
@@ -30,7 +31,7 @@ Section Progress.
   Definition Reduction_SF' := Reduction_SF P .
   Definition Reduction_FS' := Reduction_FS P .
   Definition fieldsP := fields P.
-  Definition TypeChecksP := TypeChecks P.
+  Definition TypeChecksP := TypeChecksTerm P.
   Definition Heap_okP := Heap_ok P.
   Definition Heap_dom_okP := Heap_dom_ok P .
 
@@ -40,8 +41,6 @@ Section Progress.
   Notation "( H +*+ o --> obj )" := (p_heap.updatePartFunc
                                               H o obj)
                                       (at level 0).
-
-  Print Heap_type.
 
   Definition y_dereference e y : Prop :=
     match e with
@@ -78,7 +77,7 @@ Section Progress.
                     &
                     match x_l_L with
                       | (x, l, L) => 
-                        FS = (ann_frame (sframe L (Var x))  l) :: nil
+                        FS = (ann_frame (sframe L (TVar x))  l) :: nil
                     end
       } +
 
@@ -89,13 +88,13 @@ Section Progress.
           * annotation_type
           * Env_type
           * VarName_type
-          * ExprOrTerm
-          * ExprOrTerm
+          * Expr
+          * Term
           * (list ann_frame_type)
               &
               match x_l_L_y_e_t_FS' with
                 | (x, l, L, y, e, t, FS') =>
-                  (isTerm t) /\  (isExpr e) /\ (p_env.func L y = Some envNull ) /\
+                  (p_env.func L y = Some envNull ) /\
                   (y_dereference e y) /\
                   FS = (ann_frame
                           (sframe L (
@@ -119,14 +118,13 @@ Section Progress.
     fold F in X0, X.
     destruct X0 as [sigma WF_F].
     set (WF_F'' := WF_F).
-    destruct WF_F as [H Gamma eff t' L'' ann sigma' tTerm typ_F_sigma].
+    destruct WF_F as [H Gamma eff t' L'' ann sigma' typ_F_sigma wf_h_gamma_l ].
     rename sigma' into sigma.
     clear L'.
     rename L'' into L'.
     clear t; rename t' into t.
     rename H0 into heap_okH; rename H1 into heap_dom_okH.
     destruct t.
-    induction tTerm.
     destruct ann.
     apply inl.
     apply inl.
@@ -138,7 +136,7 @@ Section Progress.
     inversion typ_F_sigma.
     clear H1 H2 H0 H4 gamma eff0 x sigma0 heap_dom_okH heap_okH X FS l .
 
-    set (w' := fst w).
+    set (w' := fst wf_h_gamma_l).
     apply (fun f => f y ) in w'.
     assert (In y (p_gamma.domain Gamma)).
     apply (p_gamma.in_part_func_domain _ _ sigma); assumption.
@@ -146,7 +144,7 @@ Section Progress.
     apply p_env.in_part_func_domain_conv; assumption.
 
     destruct X0 as [envVal L'y_eq].
-    set (G := ann_frame (sframe L' (Var y)) (ann_var v0)).
+    set (G := ann_frame (sframe L' (TVar y)) (ann_var v0)).
     fold G in X.
     destruct FS.
     apply inl.
@@ -159,18 +157,13 @@ Section Progress.
     apply E_Return1.
     assumption.
 
-    induction tTerm.
-    induction tTerm.
-    induction tTerm.
-    induction tTerm.
-    induction tTerm.
-    induction tTerm.
     rename L' into L.
-
-    set (F := ann_frame (sframe L t_let v <- t1 t_in (t2)) ann).
+    
+    rename t into t2.
+    set (F := ann_frame (sframe L t_let v <- e t_in (t2)) ann).
     fold F in X, WF_F''.
 
-    destruct t1.
+    destruct e.
     
     apply inl; apply inl.
     destruct (progress_SF_case_null
@@ -203,13 +196,13 @@ Section Progress.
     rename v0 into y.
     rename v into x.
     assert (In y (p_env.domain L)).
-    clear WF_F'' tTerm heap_okH heap_dom_okH X FS.
+    clear WF_F'' heap_okH heap_dom_okH X FS.
     inversion typ_F_sigma.
     inversion X.
     clear H9 H10 H6 H8 H7 witn f0 x1 eff1 gamma0 H2 H5 H5 H4 H3 H1 H0 X0 X t tau.
     clear x0 sigma0 e eff0 gamma.
-    apply fst in w.
-    exact (w y (p_gamma.in_part_func_domain _ _ _ H11)).
+    apply fst in wf_h_gamma_l.
+    exact (wf_h_gamma_l y (p_gamma.in_part_func_domain _ _ _ H11)).
     destruct (p_env.in_part_func_domain_conv _ _ H0).
     clear H0.
 
@@ -217,17 +210,13 @@ Section Progress.
     apply inr.
     exists (x, ann, L, y, FieldSelection y f, t2, FS).
     split.
-    inversion tTerm; assumption.
-    split.
-    simpl.
-    auto.
-    split.
     assumption.
     split.
     simpl.
-    reflexivity.
+    auto.
     reflexivity.
 
+    
     assert (p_env.func L y <> Some envNull).
     simplify_eq.
     rewrite H0 in e; discriminate.
@@ -263,15 +252,15 @@ Section Progress.
     rename v0 into y.
     rename v into x.
     assert (In y (p_env.domain L)).
-    clear WF_F'' tTerm heap_okH heap_dom_okH X FS.
+    clear WF_F'' heap_okH heap_dom_okH X FS.
     inversion typ_F_sigma.
     inversion X.
     clear H9 H10 H6 H8 H7 witn f0 x1 eff1 gamma0 H2 H5 H5 H4 H3 H1 H0 X0 X t tau H11.
     inversion X1.
     clear x0 sigma0 e eff0 gamma witn0 H5 H4 H0 H2 H1 witn f0 x1 eff1 gamma0.
-    clear H13 X1 H12 D C y0.
-    apply fst in w.
-    exact (w y (p_gamma.in_part_func_domain _ _ _ H3)).
+    clear  X1 H12 D C X2 y0.
+    apply fst in wf_h_gamma_l.
+    exact (wf_h_gamma_l y (p_gamma.in_part_func_domain _ _ _ H3)).
     destruct (p_env.in_part_func_domain_conv _ _ H0).
     clear H0.
 
@@ -279,16 +268,12 @@ Section Progress.
     apply inr.
     exists (x, ann, L, y, FieldAssignment y f v1, t2, FS).
     split.
-    inversion tTerm; assumption.
-    split.
-    simpl.
-    auto.
-    split.
     assumption.
     split.
     simpl.
+    auto.
     reflexivity.
-    reflexivity.
+
 
     assert (p_env.func L y <> Some envNull).
     simplify_eq.
@@ -323,7 +308,115 @@ Section Progress.
     assumption.
 
     (* Method invocation *)
-    admit.
+
+    rename v into x; rename v0 into y; rename v1 into z; rename t2 into t.
+
+    inversion typ_F_sigma.
+    clear H2 tau sigma t0 H5 H4 e x0 H3 eff0 H1 gamma H0 X1 typ_F_sigma
+          WF_F''
+    .
+    inversion X0.
+    rename H7 into _gamma_z_typechecks.
+    rename sigma into _gamma_z_type.
+    clear H2 z0 m0 y0 H1 H0 eff0 H4 H3  X0 H5 X1.
+
+    set (w' := fst wf_h_gamma_l).
+    assert (In z (p_env.domain L)) as z_in_L.
+    exact (w' z (p_gamma.in_part_func_domain _ _ _ _gamma_z_typechecks)).
+    clear w'.
+
+    assert (
+        (p_env.func L y = Some envNull) +
+        {o : Ref_type & p_env.func L y = Some (envRef o) /\
+             In o (p_heap.domain H)
+        }
+      ) as L_props.
+
+    clear F X  heap_dom_okH FS l heap_okH
+          ann sigma0 eff x t z _gamma_z_typechecks m md  witn gamma
+          z_in_L 
+    .
+        
+    set (w' := fst wf_h_gamma_l). 
+    set ( lem := w' y (p_gamma.in_part_func_domain _ _ _ H6)).
+    destruct (p_env.in_part_func_domain_conv _ _ lem).
+    clear lem w'.
+
+    apply snd in wf_h_gamma_l.
+    apply (fun f => f y (typt_class C) H6) in wf_h_gamma_l.
+    inversion wf_h_gamma_l.
+    destruct X.
+    apply inl; assumption.
+    destruct s; destruct x0; destruct y0; destruct p; destruct p; rewrite e0 in e.
+    apply inr.
+    exists r.
+    split; assumption.
+    destruct X. destruct x0. destruct y0. destruct p. destruct p. 
+    rewrite e1 in H6; discriminate.
+
+    destruct L_props.
+    apply inr.
+    clear l.
+    exists (x, ann, L, y, MethodInvocation y m z, t, FS).
+    split.  assumption.
+    split. reflexivity.
+    reflexivity.
+
+    destruct s as [o tmp].
+    destruct tmp as [L_y_is_o o_in_dom_H].
+    apply inl. apply inl.
+
+    apply (fun f => snd f y (typt_class C) H6) in wf_h_gamma_l.
+    destruct wf_h_gamma_l.
+    destruct s. rewrite L_y_is_o in e; discriminate.
+    destruct s; destruct x0; destruct y0; destruct p; destruct p.
+    rewrite H6 in e0; inversion e0.
+    rewrite <- H1 in *; clear c H1. 
+    clear X  gamma.
+    rewrite L_y_is_o in e; inversion e; rewrite H1 in *.
+    clear o H1; rename r into o.
+    clear o_in_dom_H  sigma0.
+    set (C' := (heap_typeof H o x0)).
+    fold C' in s.
+    unfold wf_env.subtypeP in s.
+    inversion s. clear C0 D H0 H1.
+    rename H2 into C'_sub_C.
+
+    destruct (heap_typeof_impl P _ _ C' x0 (eq_refl _)) as [FM' H_o_eq].
+    assert (method P C' m md) as m_meth_C.
+    exact (method_subclass P C' C m md witn C'_sub_C).
+    clear C  witn e0 s H6 C'_sub_C.
+    rename C' into C.
+
+    set (t' := methodBody md).
+
+    set (p := mparam P C m md m_meth_C).
+
+    destruct (p_env.in_part_func_domain_conv _ _ z_in_L) as [Lz Lz_prop].
+
+    set (L' :=                        (* L' = L[this -> o, p -> L z]*)
+                   p_env.updatePartFunc
+                     (p_env.updatePartFunc
+                        (globalEnv P)
+                        var_name_this (envRef o))
+                     p Lz).
+
+        
+    set (lem := E_Invoke P H t' t L L' x y z p m ann o C FM' FS md Lz
+                         m_meth_C   L_y_is_o 
+                         Lz_prop H_o_eq (eq_refl _)
+                         (eq_refl _) (eq_refl _)
+        ).
+
+    exists (H,
+            ann_frame (sframe L' t') (ann_var x)
+                      :: ann_frame (sframe L t) ann :: FS).
+    assumption.
+
+    destruct s; destruct x0; destruct y0; destruct p; destruct p.
+    rewrite e in L_y_is_o.
+    discriminate.
+    
 
     (* New *)
     apply inl; apply inl.
@@ -355,7 +448,6 @@ Section Progress.
 
     rename v0 into y.
     rename v1 into z.
-    destruct tTerm as [t1Term t2Term].
 
     assert (
         (p_env.func L y = Some envNull) +
@@ -364,58 +456,50 @@ Section Progress.
         }) as L_props.
       
 
-    clear F WF_F'' X t1Term t2Term heap_dom_okH FS l.
+    clear F WF_F'' X  heap_dom_okH FS l.
     inversion typ_F_sigma.
-    clear H2 tau H5 t H3 eff0 H1 gamma H0 typ_F_sigma x X0 v e H4.
+    clear H2 tau H5 H3 eff0 H1 gamma H0 typ_F_sigma x X0 v e H4 t0.
        
     inversion X.
     rewrite <- H2 in *; clear H2 H5 t H4 y0 H3 x eff0 H1 gamma H0 X1 X sigma1.
     inversion X0.
     clear H4 sigma1 H0 x H2 eff0 H1 gamma X0 sigma0 sigma eff ann.
     
-    set (w' := fst w). 
+    set (w' := fst wf_h_gamma_l). 
     set ( lem := w' y (p_gamma.in_part_func_domain _ _ _ H3)).
     destruct (p_env.in_part_func_domain_conv _ _ lem).
     clear lem w'.
 
-    apply snd in w.
-    apply (fun f => f y (typt_box C) H3) in w.
-    inversion w.
+    apply snd in wf_h_gamma_l.
+    apply (fun f => f y (typt_box C) H3) in wf_h_gamma_l.
+    inversion wf_h_gamma_l.
     destruct X.
     apply inl; assumption.
-    destruct s; destruct x0; destruct y0; destruct a; destruct H1; rewrite H1 in H3; discriminate.
-    destruct X; destruct x0; destruct y0; destruct a; destruct H1.
+    destruct s; destruct x0; destruct y0; destruct p; destruct p.  rewrite e1 in H3; discriminate.
+    destruct X; destruct x0; destruct y0; destruct p; destruct p.
     apply inr. rename r into o. exists o.
     split; assumption.
 
     destruct L_props.
     apply inr.
     clear l.
-    exists (v, ann, L, y, Open y z t1, t2, FS).
-    split. assumption.
-    split. auto.
+    exists (v, ann, L, y, Open y z t, t2, FS).
     split. assumption.
     split. reflexivity.
     reflexivity.
-    
+        
     apply inl; apply inl.
     destruct s as [o L_y_o_prop].
     exists (H,
-            (ann_frame (sframe (p_env.emptyPartFunc +++ z --> envBox o) t1) ann_epsilon) ::
+            (ann_frame (sframe (p_env.emptyPartFunc +++ z --> envBox o) t) ann_epsilon) ::
             (ann_frame (sframe ( L +++ v --> (envBox o) ) t2)
                           ann) :: FS).
     apply (E_Open P H L).
+    destruct L_y_o_prop;
     assumption.
-    assumption.
+    
     destruct L_y_o_prop.
     assumption.
-    destruct L_y_o_prop.
-    assumption.
-
-    (* let let *)
-    inversion tTerm.
-    induction H0.
-
-  Admitted.
+  Qed.
 
 End Progress.
