preservation_unfixed.v
@@ -1,0 +1,1871 @@
+Require Import syntax.
+Require Import partial.
+Require Import heap.
+Require Import classTable.
+Require Import sframe.
+Require Import reductions.
+Require Import typing.
+Require Import namesAndTypes.
+Require Import preservation.
+
+Require Import wf_env.
+
+Import ConcreteEverything.
+
+
+Section Preservation_fix.
+
+  Variable P: Program.
+
+  Definition subtypeP := subtype P.
+  Definition fldP := fld P.
+  Definition ftypeP := ftype P.
+  Definition t_frame1' := t_frame1 P.
+  Definition WF_Frame' := WF_Frame P.
+
+  Definition Reduction_SF' := Reduction_SF P .
+  Definition fieldsP := fields P.
+  Definition TypeChecksP := TypeChecksTerm P.
+  Definition TypeChecksExprP := TypeChecksExpr P.
+  Definition Heap_okP := Heap_ok P.
+  Definition Heap_dom_okP := Heap_dom_ok P .
+  
+  
+
+
+  Theorem preservation_case_new :
+    forall H L sigma ann t C x o flds,
+      WF_Frame' H (ann_frame (sframe L t_let x <- New C t_in (t)) ann) sigma ->
+      Heap_okP H ->
+      ~ In o (p_heap.domain H) ->
+      fieldsP C flds ->
+      WF_Frame'
+        (p_heap.updatePartFunc H o (obj C (p_FM.newPartFunc flds FM_null)))
+        (ann_frame (sframe (p_env.updatePartFunc L x (envRef o)) t) ann) sigma.
+    intros.
+    rename X into asm2.
+    rename H2 into H5.
+    rename H0 into asm3.
+    rename H1 into H10.
+    
+
+    (* 2 *)
+    inversion asm2.
+    rename X into _2_a.
+    rename X0 into _2_b.
+    clear H2 sigma0.
+    clear H6 ann0.
+    clear t0 H4 L0 H1 H0 H2.
+
+    (* 3 *)
+    inversion _2_b.
+    rename H0 into _3_a.
+    rename X into _3_b.
+
+    (* 4 *)
+    inversion _2_a.
+    clear tau H2 t0 H6 x0 H3 eff0 H1 gamma H0.
+    rename sigma0 into sigma'.
+    rename X0 into _4_b.
+    rename X into _4_a.
+    clear H4 e.
+
+
+    (* 5 *)
+    inversion _4_a.
+    rewrite <- H2 in *; rewrite <- H4 in *.
+    clear H1 H0 C0 H2 H4 H2 eff.
+    rename H3 into C_is_ocap.
+
+
+    (* section between 5, 6 let's call it half_6 *)
+    (* This is not in the same order on paper *)
+    (* split. *)
+    apply ( t_frame1' _
+                      (p_gamma.updatePartFunc Gamma x (typt_class C))
+                      eff_ocap _ _ ann sigma).
+    exact H5.
+    exact _4_b.
+    assert (gamma_env_subset (p_gamma.updatePartFunc Gamma x (typt_class C))
+                             (p_env.updatePartFunc L x (envRef o))) as _7.
+    exact (subset_preserved Gamma L x sigma' envNull _3_a). (* actually, 7 *)
+    split. exact _7.
+    intros z tau.
+    case_eq (v_eq_dec x z).
+    intro x_is_z; rewrite <- x_is_z in *; clear x_is_z z.
+    intro dummy; clear dummy.
+    (* Section half 6 on paper here somewhere *)
+    intro half_6.
+    set (half_6_a_i := proj1 (p_env.updatedFuncProp L x (envRef o) x) (eq_refl _)).
+    assert (In o (p_heap.domain (p_heap.updatePartFunc H o (obj C (p_FM.newPartFunc flds FM_null)))))
+      as o_witn.
+    apply p_heap.updatedFuncIn.
+    set (H'o := proj1 (p_heap.updatedFuncProp H o (obj C (p_FM.newPartFunc flds FM_null)) o)
+                      (eq_refl _)).
+    assert ((heap_typeof
+               (p_heap.updatePartFunc H o
+                                      (obj C (p_FM.newPartFunc flds FM_null)))
+               o o_witn) = C) as half_6_a_ii_first.
+    apply (heap_typeof_same P _ _ _ _ H'o).
+    
+    (* rewrite e. *)
+    (* reflexivity. *)
+
+    
+    assert (subtypeP ( typt_class (heap_typeof
+                                     (p_heap.updatePartFunc H o
+                                                            (obj C (p_FM.newPartFunc flds FM_null)))
+                                     o o_witn)) (typt_class C)) as half_6_a_ii.
+    rewrite half_6_a_ii_first.
+    unfold subtypeP.
+    apply classSub.
+    apply subclass_refl. (* admitted (actually not defined) *)
+    set (lem := proj1 (p_gamma.updatedFuncProp Gamma x (typt_class C) x) (eq_refl _)).
+    rewrite half_6 in lem.
+    inversion lem.
+    rewrite H1 in *; clear lem H1 tau.
+    rename half_6 into half_6_a_iii.
+    apply inl. apply inr. exists (C, o).
+    exists o_witn.
+    split. split.
+    exact half_6_a_i.
+    
+    exact half_6_a_iii.
+    exact half_6_a_ii.
+
+    (* 6 [THIS starts like #4 from E-Null]*)
+    
+    intros _6_c dummy _6_a.
+    clear dummy.
+    
+    
+    assert (p_gamma.func Gamma z = Some tau) as e_vi.
+    rewrite <- _6_a.
+    symmetry.
+    apply (proj2 (p_gamma.updatedFuncProp Gamma x (typt_class C) z)).
+    firstorder.
+    
+    (* set (new__4_d := _6_b z tau _4_a). *)
+    (* unfold WF_Var. *)
+    
+    (* rewrite H0. *)
+    
+
+    
+    (* Require Import Coq.Lists.List. *)
+    assert (In z (p_gamma.domain Gamma)) as z_in_dom_Gamma.
+    set (lem := p_gamma.fDomainCompat Gamma z).
+    set (in_or_not := in_dec v_eq_dec z (p_gamma.domain Gamma)).
+    firstorder. rewrite H0 in e_vi; discriminate.
+
+    
+
+    set (z_in_dom_L := _3_a z z_in_dom_Gamma).
+    case_eq (p_env.func L z).
+    intros envVar L_z_val.
+    assert (p_env.func (p_env.updatePartFunc L x (envRef o) ) z = Some envVar) as _6_bb.
+    transitivity (p_env.func L z).
+    apply p_env.updatedFuncProp. firstorder.
+    exact L_z_val.
+
+    destruct envVar.
+
+    (* 6 d *)
+    apply inl. apply inl.
+    exact _6_bb.
+
+    (* 6 e *)
+    
+    rename r into o'.
+
+    assert ({ C : _ &  {witn : _ &
+                                 (p_env.func L z = Some (envRef o')) *
+                               (p_gamma.func Gamma z = Some (typt_class C)) *
+                               subtypeP (typt_class (heap_typeof H o' witn)) (typt_class C)
+                       }}).
+    elim (_3_b z tau e_vi).
+    intro.
+    destruct a.
+    rewrite -> e in L_z_val; discriminate.
+    destruct s.
+    destruct x0.
+    destruct y.
+    destruct p.
+    destruct p.
+    rewrite L_z_val in H0.
+    inversion H0.
+    rewrite H4 in *; clear H4 o'; rename r into o'.
+    clear H0.
+    rewrite e_vi in H1.
+    inversion H1. rewrite -> H3 in *.
+    clear H3 tau H1.
+    exists c. exists x0.
+    split.
+    exact L_z_val.
+    split.
+    exact e_vi.
+    exact H2.
+
+    intro.
+    destruct b. destruct x0. destruct y. destruct a. destruct H1.
+    exists c.
+    rewrite L_z_val in H0.
+    inversion H0.
+    destruct X. destruct s. destruct a. destruct H1.
+    clear H0.
+    rename x0 into C'.
+    rename x1 into o'_witness.
+
+    apply inl. apply inr.
+    exists (C', o').
+    exists (p_heap.staysInDomain H o (obj C (p_FM.newPartFunc flds FM_null)) o' o'_witness).
+    split.
+    exact _6_bb.
+    split.
+    rewrite <- H1.
+    apply (p_gamma.updatedFuncProp). firstorder.
+
+    set (H' := (p_heap.updatePartFunc H o (obj C (p_FM.newPartFunc flds FM_null)))).
+    apply classSub.
+    inversion H2.
+    assert (p_heap.func H o' = p_heap.func H' o') as _6_e_ii.
+    apply (p_heap.freshProp _ _ _ H10 _ o'_witness).
+    assert ((heap_typeof H' o'
+                         (p_heap.staysInDomain H o (obj C (p_FM.newPartFunc flds FM_null)) o'
+                                               o'_witness))
+            = (heap_typeof H o' o'_witness))
+      as _6_e_iii.
+
+    case_eq (p_heap.func H o').
+    intros. destruct b.
+    set (stays_witn := (p_heap.staysInDomain
+                          H o
+                          (obj C
+                               (p_FM.newPartFunc flds FM_null)) o'
+                          o'_witness)).
+    fold stays_witn.
+    rewrite <- H0 in *.
+    rewrite _6_e_ii in H6.
+    assert (c = C0).
+    symmetry in H0.
+    set (lem := heap_typeof_impl P _ _ _ _ H0).
+    destruct lem.
+    rewrite H6 in _6_e_ii.
+    rewrite e in _6_e_ii.
+    inversion _6_e_ii.
+    reflexivity.
+    rewrite <- H8.
+    apply (heap_typeof_same P _ _ _ _ H6).
+
+    (* None *)
+    intro is_none;  induction (proj2 (p_heap.fDomainCompat _ _)
+                                     is_none o'_witness).
+    
+    rewrite _6_e_iii.
+    exact H4.
+    
+    (* 6 L(z) = box o' *)
+    rename r into o'.
+    set (H' := (p_heap.updatePartFunc H o (obj C (p_FM.newPartFunc flds FM_null)))).
+    set (Gamma' := (p_gamma.updatePartFunc Gamma x (typt_class C))).
+    fold Gamma' in _4_b, _7, _6_a.
+    set (L' := (p_env.updatePartFunc L x (envRef o))).
+    fold L' in _7, _6_bb.
+
+    set (o_is_WF := _3_b z tau e_vi).
+    inversion o_is_WF.
+    destruct X.
+    rewrite e in L_z_val.
+    inversion L_z_val.
+    destruct s.
+    destruct x0.
+    destruct y.
+    destruct a.
+    rewrite H0 in L_z_val.
+    inversion L_z_val.
+
+    destruct X.  destruct x0.    destruct y. destruct a. destruct H1.
+    rewrite H0 in L_z_val.
+    inversion L_z_val.
+    rewrite <- H4 in *.
+    clear o' H4.
+    rename r into o'.
+    clear L_z_val.
+    apply inr.
+    exists (c, o').
+    exists (p_heap.staysInDomain _ _ _ _ x0).
+    split.
+    rewrite <- H0.
+    apply (proj2 (p_env.updatedFuncProp _ _  _ _ )).
+    firstorder.
+    split.
+    rewrite <- H1.
+    apply (proj2 (p_gamma.updatedFuncProp _ _  _ _ )).
+    firstorder.
+    apply classSub.
+    inversion H2.
+    clear H4 C0 H3.
+    assert (p_heap.func H o' = p_heap.func H' o').
+    apply (p_heap.freshProp).
+    exact H10.
+    exact x0.
+
+    set (C' :=  heap_typeof H o' x0).
+    fold C' in H6, H2.
+    set (stays_witn := (p_heap.staysInDomain
+                          H o (obj C (p_FM.newPartFunc flds FM_null)) o'
+                          x0)).
+    assert ((heap_typeof H' o' stays_witn) = C').
+
+    destruct (heap_typeof_impl P _ _ C' x0 (eq_refl _)).
+    rewrite e in H3.
+    symmetry in H3.
+    apply (heap_typeof_same P _ _ _ _ H3 stays_witn).
+    rewrite H4.
+    assumption.
+    intro L_z_is_none; induction (proj2 (p_env.fDomainCompat _ _) L_z_is_none).
+    auto.
+
+
+    (*** effect EPSILON ***)
+    rewrite <- H2 in *;
+      rewrite <- H1 in *.
+    clear H1 H0 C0 H2 H2 eff H3.
+    
+
+    (* section between 5, 6 let's call it half_6 *)
+    (* This is not in the same order on paper *)
+    (* split. *)
+    apply ( t_frame1' _
+                      (p_gamma.updatePartFunc Gamma x (typt_class C))
+                      eff_epsilon _ _ ann sigma).
+    exact H5.
+    exact _4_b.
+    assert (gamma_env_subset (p_gamma.updatePartFunc Gamma x (typt_class C))
+                             (p_env.updatePartFunc L x (envRef o))) as _7.
+    exact (subset_preserved Gamma L x sigma' envNull _3_a). (* actually, 7 *)
+    split. exact _7.
+    intros z tau.
+    case_eq (v_eq_dec x z).
+    intro x_is_z; rewrite <- x_is_z in *; clear x_is_z z.
+    intro dummy; clear dummy.
+    (* Section half 6 on paper here somewhere *)
+    intro half_6.
+    set (half_6_a_i := proj1 (p_env.updatedFuncProp L x (envRef o) x) (eq_refl _)).
+    assert (In o (p_heap.domain (p_heap.updatePartFunc H o (obj C (p_FM.newPartFunc flds FM_null)))))
+      as o_witn.
+    apply p_heap.updatedFuncIn.
+    set (H'o := proj1 (p_heap.updatedFuncProp H o (obj C (p_FM.newPartFunc flds FM_null)) o)
+                      (eq_refl _)).
+    assert ((heap_typeof
+               (p_heap.updatePartFunc H o
+                                      (obj C (p_FM.newPartFunc flds FM_null)))
+               o o_witn) = C) as half_6_a_ii_first.
+    apply (heap_typeof_same P _ _ _ _ H'o).
+    
+    (* rewrite e. *)
+    (* reflexivity. *)
+
+    
+    assert (subtypeP ( typt_class (heap_typeof
+                                     (p_heap.updatePartFunc H o
+                                                            (obj C (p_FM.newPartFunc flds FM_null)))
+                                     o o_witn)) (typt_class C)) as half_6_a_ii.
+    rewrite half_6_a_ii_first.
+    unfold subtypeP.
+    apply classSub.
+    apply subclass_refl. 
+    set (lem := proj1 (p_gamma.updatedFuncProp Gamma x (typt_class C) x) (eq_refl _)).
+    rewrite half_6 in lem.
+    inversion lem.
+    rewrite H1 in *; clear lem H1 tau.
+    rename half_6 into half_6_a_iii.
+    apply inl. apply inr. exists (C, o).
+    exists o_witn.
+    split.
+    exact half_6_a_i.
+    split.
+    exact half_6_a_iii.
+    exact half_6_a_ii.
+
+    (* 6 [THIS starts like #4 from E-Null]*)
+    
+    intros _6_c dummy _6_a.
+    clear dummy.
+    
+    
+    assert (p_gamma.func Gamma z = Some tau) as e_vi.
+    rewrite <- _6_a.
+    symmetry.
+    apply (proj2 (p_gamma.updatedFuncProp Gamma x (typt_class C) z)).
+    firstorder.
+    
+    (* set (new__4_d := _6_b z tau _4_a). *)
+    (* unfold WF_Var. *)
+    
+    (* rewrite H0. *)
+    
+
+    
+    (* Require Import Coq.Lists.List. *)
+    assert (In z (p_gamma.domain Gamma)) as z_in_dom_Gamma.
+    set (lem := p_gamma.fDomainCompat Gamma z).
+    set (in_or_not := in_dec v_eq_dec z (p_gamma.domain Gamma)).
+    firstorder. rewrite H0 in e_vi; discriminate.
+
+    
+
+    set (z_in_dom_L := _3_a z z_in_dom_Gamma).
+    case_eq (p_env.func L z).
+    intros envVar L_z_val.
+    assert (p_env.func (p_env.updatePartFunc L x (envRef o) ) z = Some envVar) as _6_bb.
+    transitivity (p_env.func L z).
+    apply p_env.updatedFuncProp. firstorder.
+    exact L_z_val.
+
+    destruct envVar.
+
+    (* 6 d *)
+    apply inl. apply inl.
+    exact _6_bb.
+
+    (* 6 e *)
+    
+    rename r into o'.
+
+    assert ({ C | {witn |
+                   p_env.func L z = Some (envRef o') /\
+                   p_gamma.func Gamma z = Some (typt_class C) /\
+                   subtypeP (typt_class (heap_typeof H o' witn)) (typt_class C)
+                  }}).
+    elim (_3_b z tau e_vi).
+    intro.
+    destruct a.
+    rewrite -> e in L_z_val; discriminate.
+    destruct s.
+    destruct x0.
+    destruct y.
+    destruct a.
+    destruct H1.
+    rewrite L_z_val in H0.
+    inversion H0.
+    rewrite H4 in *; clear H4 o'; rename r into o'.
+    clear H0.
+    rewrite e_vi in H1.
+    inversion H1. rewrite -> H3 in *.
+    clear H3 tau H1.
+    exists c. exists x0.
+    split.
+    exact L_z_val.
+    split.
+    exact e_vi.
+    exact H2.
+
+    intro.
+    destruct b. destruct x0. destruct y. destruct a. destruct H1.
+    exists c.
+    rewrite L_z_val in H0.
+    inversion H0.
+    destruct X. destruct s. destruct a. destruct H1.
+    clear H0.
+    rename x0 into C'.
+    rename x1 into o'_witness.
+
+    apply inl. apply inr.
+    exists (C', o').
+    exists (p_heap.staysInDomain H o (obj C (p_FM.newPartFunc flds FM_null)) o' o'_witness).
+    split.
+    exact _6_bb.
+    split.
+    rewrite <- H1.
+    apply (p_gamma.updatedFuncProp). firstorder.
+
+    set (H' := (p_heap.updatePartFunc H o (obj C (p_FM.newPartFunc flds FM_null)))).
+    apply classSub.
+    inversion H2.
+    assert (p_heap.func H o' = p_heap.func H' o') as _6_e_ii.
+    apply (p_heap.freshProp _ _ _ H10 _ o'_witness).
+    assert ((heap_typeof H' o'
+                         (p_heap.staysInDomain H o (obj C (p_FM.newPartFunc flds FM_null)) o'
+                                               o'_witness))
+            = (heap_typeof H o' o'_witness))
+      as _6_e_iii.
+
+    case_eq (p_heap.func H o').
+    intros. destruct b.
+    set (stays_witn := (p_heap.staysInDomain
+                          H o
+                          (obj C
+                               (p_FM.newPartFunc flds FM_null)) o'
+                          o'_witness)).
+    fold stays_witn.
+    rewrite <- H0 in *.
+    rewrite _6_e_ii in H6.
+    assert (c = C0).
+    symmetry in H0.
+    set (lem := heap_typeof_impl P _ _ _ _ H0).
+    destruct lem.
+    rewrite H6 in _6_e_ii.
+    rewrite e in _6_e_ii.
+    inversion _6_e_ii.
+    reflexivity.
+    rewrite <- H8.
+    apply (heap_typeof_same P _ _ _ _ H6).
+
+    (* None *)
+    intro is_none;  induction (proj2 (p_heap.fDomainCompat _ _)
+                                     is_none o'_witness).
+    
+    rewrite _6_e_iii.
+    exact H4.
+    
+    (* 6 L(z) = box o' *)
+    rename r into o'.
+    set (H' := (p_heap.updatePartFunc H o (obj C (p_FM.newPartFunc flds FM_null)))).
+    set (Gamma' := (p_gamma.updatePartFunc Gamma x (typt_class C))).
+    fold Gamma' in _4_b, _7, _6_a.
+    set (L' := (p_env.updatePartFunc L x (envRef o))).
+    fold L' in _7, _6_bb.
+
+    set (o_is_WF := _3_b z tau e_vi).
+    inversion o_is_WF.
+    destruct X.
+    rewrite e in L_z_val.
+    inversion L_z_val.
+    destruct s.
+    destruct x0.
+    destruct y.
+    destruct a.
+    rewrite H0 in L_z_val.
+    inversion L_z_val.
+
+    destruct X.  destruct x0.    destruct y. destruct a. destruct H1.
+    rewrite H0 in L_z_val.
+    inversion L_z_val.
+    rewrite <- H4 in *.
+    clear o' H4.
+    rename r into o'.
+    clear L_z_val.
+    apply inr.
+    exists (c, o').
+    exists (p_heap.staysInDomain _ _ _ _ x0).
+    split.
+    rewrite <- H0.
+    apply (proj2 (p_env.updatedFuncProp _ _  _ _ )).
+    firstorder.
+    split.
+    rewrite <- H1.
+    apply (proj2 (p_gamma.updatedFuncProp _ _  _ _ )).
+    firstorder.
+    apply classSub.
+    inversion H2.
+    clear H4 C0 H3.
+    assert (p_heap.func H o' = p_heap.func H' o').
+    apply (p_heap.freshProp).
+    exact H10.
+    exact x0.
+    
+    (* TODO: find out why it doesn't work! *)
+    set (C' :=  heap_typeof H o' x0).
+    fold C' in H6, H2.
+    set (stays_witn := (p_heap.staysInDomain
+                          H o (obj C (p_FM.newPartFunc flds FM_null)) o'
+                          x0)).
+    assert ((heap_typeof H' o' stays_witn) = C').
+
+    destruct (heap_typeof_impl P _ _ C' x0 (eq_refl _)).
+    rewrite e in H3.
+    symmetry in H3.
+    apply (heap_typeof_same P _ _ _ _ H3 stays_witn).
+    rewrite H4.
+    assumption.
+
+    intro L_z_is_none; induction (proj2 (p_env.fDomainCompat _ _) L_z_is_none).
+    auto.
+  Qed.
+
+  Theorem preservation_case_box :
+    forall H L sigma ann t C x o flds,
+      WF_Frame' H (ann_frame (sframe L t_let x <- Box C t_in (t)) ann) sigma ->
+      Heap_okP H ->
+      ~ In o (p_heap.domain H) ->
+      fieldsP C flds ->
+      WF_Frame'
+        (p_heap.updatePartFunc H o (obj C (p_FM.newPartFunc flds FM_null)))
+        (ann_frame (sframe (p_env.updatePartFunc L x (envBox o)) t) ann) sigma.
+    intros.
+    rename X into asm2.
+    rename H2 into H5.
+    rename H0 into asm3.
+    rename H1 into H10.
+    
+
+    (* 2 *)
+    inversion asm2.
+    rename X into _2_a.
+    rename X0 into _2_b.
+    clear H2 sigma0.
+    clear H6 ann0.
+    clear t0 H4 L0 H1 H0 H3.
+
+    (* 3 *)
+    inversion _2_b.
+    rename H0 into _3_a.
+    rename X into _3_b.
+
+    (* 4 *)
+    inversion _2_a.
+    clear tau H2 t0 H6 x0 H3 eff0 H1 gamma H0.
+    rename sigma0 into sigma'.
+    rename X0 into _4_b.
+    rename X into _4_a.
+    clear H4 e.
+
+
+    (* 5 *)
+    inversion _4_a.
+    rewrite <- H2 in *; rewrite <- H4 in *.
+    clear H1 H0 C0 H2 H4 H2 eff.
+    rename H3 into C_is_ocap.
+
+
+    (* section between 5, 6 let's call it half_6 *)
+    (* This is not in the same order on paper *)
+    (* split. *)
+    apply ( t_frame1' _
+                     (p_gamma.updatePartFunc Gamma x (typt_box C))
+                     eff_ocap _ _ ann sigma).
+    exact _4_b.
+    assert (gamma_env_subset (p_gamma.updatePartFunc Gamma x (typt_box C))
+     (p_env.updatePartFunc L x (envBox o))) as _7.
+    exact (subset_preserved Gamma L x sigma' envNull _3_a). (* actually, 7 *)
+    split. exact _7.
+    intros z tau.
+    case_eq (v_eq_dec x z).
+    intro x_is_z; rewrite <- x_is_z in *; clear x_is_z z.
+    intro dummy; clear dummy.
+    (* Section half 6 on paper here somewhere *)
+    intro half_6.
+    set (half_6_a_i := proj1 (p_env.updatedFuncProp L x (envBox o) x) (eq_refl _)).
+    assert (In o (p_heap.domain (p_heap.updatePartFunc H o (obj C (p_FM.newPartFunc flds FM_null)))))
+      as o_witn.
+    apply p_heap.updatedFuncIn.
+    set (H'o := proj1 (p_heap.updatedFuncProp H o (obj C (p_FM.newPartFunc flds FM_null)) o)
+                      (eq_refl _)).
+    assert ((heap_typeof
+               (p_heap.updatePartFunc H o
+                                      (obj C (p_FM.newPartFunc flds FM_null)))
+               o o_witn) = C) as half_6_a_ii_first.
+    apply (heap_typeof_same P _ _ _ _ H'o).
+    
+    (* rewrite e. *)
+    (* reflexivity. *)
+
+    
+    assert (subtypeP ( typt_class (heap_typeof
+                                     (p_heap.updatePartFunc H o
+                                                            (obj C (p_FM.newPartFunc flds FM_null)))
+                                     o o_witn)) (typt_class C)) as half_6_a_ii.
+    rewrite half_6_a_ii_first.
+    unfold subtypeP.
+    apply classSub.
+    apply subclass_refl. 
+    set (lem := proj1 (p_gamma.updatedFuncProp Gamma x (typt_box C) x) (eq_refl _)).
+    rewrite half_6 in lem.
+    inversion lem.
+    rewrite H1 in *; clear lem H1 tau.
+    rename half_6 into half_6_a_iii.
+    apply inr.  exists (C, o).
+    exists o_witn.
+    split. split.
+    exact half_6_a_i.
+    exact half_6_a_iii.
+    exact half_6_a_ii.
+
+    (* 6 [THIS starts like #4 from E-Null]*)
+    
+    intros _6_c dummy _6_a.
+    clear dummy.
+    
+        
+    assert (p_gamma.func Gamma z = Some tau) as e_vi.
+    rewrite <- _6_a.
+    symmetry.
+    apply (proj2 (p_gamma.updatedFuncProp Gamma x (typt_box C) z)).
+    firstorder.
+    
+    (* set (new__4_d := _6_b z tau _4_a). *)
+    (* unfold WF_Var. *)
+    
+    (* rewrite H0. *)
+    
+
+    
+    (* Require Import Coq.Lists.List. *)
+    assert (In z (p_gamma.domain Gamma)) as z_in_dom_Gamma.
+    set (lem := p_gamma.fDomainCompat Gamma z).
+    set (in_or_not := in_dec v_eq_dec z (p_gamma.domain Gamma)).
+    firstorder. rewrite H0 in e_vi; discriminate.
+
+    
+
+    set (z_in_dom_L := _3_a z z_in_dom_Gamma).
+    case_eq (p_env.func L z).
+    intros envVar L_z_val.
+    assert (p_env.func (p_env.updatePartFunc L x (envBox o) ) z
+            = Some envVar) as _6_bb.
+    transitivity (p_env.func L z).
+    apply p_env.updatedFuncProp. firstorder.
+    exact L_z_val.
+
+    destruct envVar.
+
+    (* 6 d *)
+    apply inl. apply inl.
+    exact _6_bb.
+
+    (* 6 e *)
+    
+    rename r into o'.
+
+    assert ({ C : _ & {witn : _ &
+             (p_env.func L z = Some (envRef o')) *
+             (p_gamma.func Gamma z = Some (typt_class C)) *
+             subtypeP (typt_class (heap_typeof H o' witn)) (typt_class C)
+            }}).
+    elim (_3_b z tau e_vi).
+    intro.
+    destruct a.
+    rewrite -> e in L_z_val; discriminate.
+    destruct s.
+    destruct x0.
+    destruct y.
+    destruct a.
+    destruct H1.
+    rewrite L_z_val in H0.
+    inversion H0.
+    rewrite H4 in *; clear H4 o'; rename r into o'.
+    clear H0.
+    rewrite e_vi in H1.
+    inversion H1. rewrite -> H3 in *.
+    clear H3 tau H1.
+    exists c. exists x0.
+    split.
+    exact L_z_val.
+    split.
+    exact e_vi.
+    exact H2.
+
+    intro.
+    destruct b. destruct x0. destruct y. destruct a. destruct H1.
+    exists c.
+    rewrite L_z_val in H0.
+    inversion H0.
+    destruct X. destruct s. destruct a. destruct H1.
+    clear H0.
+    rename x0 into C'.
+    rename x1 into o'_witness.
+
+    apply inl. apply inr.
+    exists (C', o').
+    exists (p_heap.staysInDomain H o (obj C (p_FM.newPartFunc flds FM_null)) o' o'_witness).
+    split.
+    exact _6_bb.
+    split.
+    rewrite <- H1.
+    apply (p_gamma.updatedFuncProp). firstorder.
+
+    set (H' := (p_heap.updatePartFunc H o (obj C (p_FM.newPartFunc flds FM_null)))).
+    apply classSub.
+    inversion H2.
+    assert (p_heap.func H o' = p_heap.func H' o') as _6_e_ii.
+    apply (p_heap.freshProp _ _ _ H10 _ o'_witness).
+    assert ((heap_typeof H' o'
+                         (p_heap.staysInDomain H o (obj C (p_FM.newPartFunc flds FM_null)) o'
+                                               o'_witness))
+            = (heap_typeof H o' o'_witness))
+      as _6_e_iii.
+
+    case_eq (p_heap.func H o').
+    intros. destruct b.
+    set (stays_witn := (p_heap.staysInDomain
+                          H o
+                          (obj C
+                               (p_FM.newPartFunc flds FM_null)) o'
+                          o'_witness)).
+    fold stays_witn.
+    rewrite <- H0 in *.
+    rewrite _6_e_ii in H6.
+    assert (c = C0).
+    symmetry in H0.
+    set (lem := heap_typeof_impl P _ _ _ _ H0).
+    destruct lem.
+    rewrite H6 in _6_e_ii.
+    rewrite e in _6_e_ii.
+    inversion _6_e_ii.
+    reflexivity.
+    rewrite <- H8.
+    apply (heap_typeof_same P _ _ _ _ H6).
+
+    (* None *)
+    intro is_none;  induction (proj2 (p_heap.fDomainCompat _ _)
+                                     is_none o'_witness).
+        
+    rewrite _6_e_iii.
+    exact H4.
+    
+    (* 6 L(z) = box o' *)
+    rename r into o'.
+    set (H' := (p_heap.updatePartFunc H o (obj C (p_FM.newPartFunc flds FM_null)))).
+    set (Gamma' := (p_gamma.updatePartFunc Gamma x (typt_class C))).
+    fold Gamma' in _4_b, _7, _6_a.
+    set (L' := (p_env.updatePartFunc L x (envRef o))).
+    fold L' in _7, _6_bb.
+
+    set (o_is_WF := _3_b z tau e_vi).
+    inversion o_is_WF.
+    destruct X.
+    rewrite e in L_z_val.
+    inversion L_z_val.
+    destruct s.
+    destruct x0.
+    destruct y.
+    destruct a.
+    rewrite H0 in L_z_val.
+    inversion L_z_val.
+
+    destruct X.  destruct x0.    destruct y. destruct a. destruct H1.
+    rewrite H0 in L_z_val.
+    inversion L_z_val.
+    rewrite <- H4 in *.
+    clear o' H4.
+    rename r into o'.
+    clear L_z_val.
+    apply inr.
+    exists (c, o').
+    exists (p_heap.staysInDomain _ _ _ _ x0).
+    split.
+    rewrite <- H0.
+    apply (proj2 (p_env.updatedFuncProp _ _  _ _ )).
+    firstorder.
+    split.
+    rewrite <- H1.
+    apply (proj2 (p_gamma.updatedFuncProp _ _  _ _ )).
+    firstorder.
+    apply classSub.
+    inversion H2.
+    clear H4 C0 H3.
+    assert (p_heap.func H o' = p_heap.func H' o').
+    apply (p_heap.freshProp).
+    exact H10.
+    exact x0.
+
+    set (C' :=  heap_typeof H o' x0).
+    fold C' in H6, H2.
+    set (stays_witn := (p_heap.staysInDomain
+                          H o (obj C (p_FM.newPartFunc flds FM_null)) o'
+                          x0)).
+    assert ((heap_typeof H' o' stays_witn) = C').
+
+    destruct (heap_typeof_impl P _ _ C' x0 (eq_refl _)).
+    rewrite e in H3.
+    symmetry in H3.
+    apply (heap_typeof_same P _ _ _ _ H3 stays_witn).
+    rewrite H4.
+    assumption.
+    intro L_z_is_none; induction (proj2 (p_env.fDomainCompat _ _) L_z_is_none).
+    auto.
+  Qed.
+
+    Theorem preservation_case_select :
+    forall H L sigma ann x y f t C FM fmVal o,
+      WF_Frame' H (ann_frame (sframe L t_let x <- FieldSelection y f t_in (t)) ann) sigma ->
+      Heap_okP H ->
+      p_env.func L y = Some (envRef o) ->
+      p_heap.func H o = Some (obj C FM) ->
+      p_FM.func FM f = Some fmVal ->
+      WF_Frame'
+        H
+        (ann_frame (sframe (p_env.updatePartFunc L x (fm2env fmVal)) t) ann) sigma.
+    intros.
+
+    (* 2 *)
+    rename H1 into _2_ab.
+    rename H2 into _2_cd.
+    rename H3 into _2_e.
+    rename H4 into t_is_term.
+    rename H0 into _2_j.
+    rename X into _2_k.
+
+    (* 3 *)
+    inversion _2_k.
+    clear H3 sigma0 H5 ann0 H4 H1 H2.
+    rename X into _3_a.
+    rename X0 into _3_b.
+
+
+    (* 4 *)
+    inversion _3_a.
+    clear tau H3 H7 t1 H5 e H4 x0 eff0 H2.
+    rewrite <- H1 in * ; clear H1 Gamma.
+    inversion X.
+    clear H5 f0 H1 x0 eff0 H3 gamma0 H2.
+    rename C0 into D.
+    rename H7 into _4_a.
+    rename witn into _4_b.
+    set (E := ftype P D f _4_b).
+    rewrite <- H4 in *.
+    fold E in X, X0.
+    clear H4.
+    (* rename H4 into _4_c. *)
+    rename X0 into _4_d.
+    rename X into _4_e.
+    set (L' := p_env.updatePartFunc L x (fm2env fmVal)).
+    clear t0 L0 H0.
+
+
+    (* 5 *)
+    set (Gamma' := p_gamma.updatePartFunc gamma x (typt_class E)).
+    fold Gamma' in _4_d.
+    
+    (* 6 *)
+    inversion _3_b.
+    rename H0 into _3_b_i.
+    rename X into _3_b_ii.
+    set (_6 := subset_preserved gamma L x (typt_class E) (fm2env fmVal)  _3_b_i).
+
+
+    (* OTHER ORDER COMPARED TO paper proof*)
+    clear H6 sigma0.
+    apply (t_frame1 P _ Gamma' eff _ _ _ _ t_is_term _4_d).
+    split.
+    apply _6.
+    intros z tau.
+
+    (* END OTHER *)
+
+    case_eq (v_eq_dec x z).
+    (* 7 *)
+    (* 7 a *)
+    intros.
+    rewrite <- e in *; clear e z.
+    clear H0.
+    assert (p_env.func L' x = Some (fm2env fmVal)) as _7_a.
+    unfold L'.
+    rewrite  ( proj1 (p_env.updatedFuncProp L x (fm2env fmVal) x) (eq_refl x)).
+    reflexivity.
+    
+    assert (p_gamma.func Gamma' x = Some (typt_class E)) as gamma_x_E.
+    unfold Gamma'.
+    rewrite  ( proj1 (p_gamma.updatedFuncProp gamma x (typt_class E) x) (eq_refl x)).
+    reflexivity.
+    clear H1.
+
+    (* 7 b *)
+    induction fmVal; unfold fm2env in _7_a.
+    
+    (* 7 b i *)
+    apply inl. apply inl.
+    exact _7_a.
+
+    (* 7 c *)
+    rename r into o'.
+    set (test := _2_j o C FM _2_cd f o').
+    
+    apply inl.  apply inr.
+    exists (E, o').
+    unfold Gamma'.
+    assert (subclass P C D) as C_sub_D.
+    
+    induction ( _3_b_ii y (typt_class D) _4_a).
+    induction a.
+    rewrite  _2_ab in a; discriminate a.
+    destruct b.
+    destruct x0.
+    destruct y0.
+    destruct a.
+    destruct H1.
+    rewrite _2_ab in H0.
+    inversion H0.
+    rewrite H4 in *.
+    rewrite _4_a in H1.
+    inversion H1.
+    rewrite <- H5 in *.
+    clear c H5.
+    assert (heap_typeof H r x0 = C).
+    unfold heap_typeof.
+    (* TODO: rewriting *)
+    admit.
+    (* rewrite <- H4. *)
+    (* rewrite _2_cd. *)
+    (* reflexivity. *)
+    rewrite H3 in H2.
+    inversion H2.
+    exact H7.
+    destruct b.   destruct x0. 
+    destruct y0.
+    destruct a.
+    rewrite _2_ab in H0.
+    inversion H0.
+    
+    assert (fld P C f) as f_field_C.
+    apply (field_subclass P C D  _  _4_b).
+    
+    exact C_sub_D.
+    destruct (test f_field_C _2_e).
+    clear test.
+    exists x0.
+    split.
+    exact _7_a.
+    split.
+    exact gamma_x_E.
+    
+    (*  *)
+    (*
+     * know: Gamma' x = E
+     * typeof(H, o') <: ftype(C, f)
+     * --------------
+     * ftype(C, f) = E
+     * --------------------- 
+     * Goal:  heapof(H, o') <: E
+     *
+     *)
+    apply classSub.
+    assert (E = heap.ftypeP P C f f_field_C).
+    unfold E.
+    unfold heap.ftypeP.
+    rewrite (unique_ftype P C f f_field_C (field_subclass P C D f f_field_C C_sub_D)).
+    rewrite <- (ftype_subclass P C D f f_field_C C_sub_D).
+    apply (unique_ftype P D f _ _).
+    rewrite <- H0 in s.
+    exact s.
+
+    (* 8 *)
+    intros.
+    clear H0.
+
+    (* 8 a b *)
+    assert (p_gamma.func gamma z = Some tau).
+    rewrite <- H1.
+    symmetry.
+    set (lem := proj2 (p_gamma.updatedFuncProp gamma x (typt_class E) z)).
+    firstorder.
+    rename H0 into _8_b.
+    assert (In z (p_gamma.domain gamma)) as _8_a.
+    apply (p_gamma.in_part_func_domain _ z tau _8_b).
+
+    (* 8 c *)
+    assert (In z (p_env.domain L)) as _8_c.
+    apply (_3_b_i _ _8_a).
+
+    set (_8_e_i := _3_b_ii z tau _8_b).
+    unfold WF_Var.
+
+    assert (p_env.func L z = p_env.func L' z) as _8_d.
+    set (lem := proj2 (p_env.updatedFuncProp L x (fm2env fmVal) z)).
+    symmetry. firstorder.
+    rewrite <- _8_d.
+    rewrite <- _8_b in H1.
+    rewrite H1.
+    exact _8_e_i.
+  Admitted.
+
+
+    Theorem preservation_case_assign H L x y f z t C FM o sigma envVal ann:
+    forall witn: is_not_box envVal,
+      WF_Frame' H (ann_frame (sframe L t_let x <- (FieldAssignment y f z) t_in (t)) ann) sigma ->
+      Heap_okP H ->
+      p_env.func L y = Some (envRef o) ->
+      p_heap.func H o = Some (obj C FM) ->
+      p_env.func L z = Some envVal ->
+      (* isTerm t -> *)
+      (WF_Frame'
+         (p_heap.updatePartFunc H o
+                                (obj C (p_FM.updatePartFunc FM f (env2fm envVal witn))))
+         (ann_frame (sframe (p_env.updatePartFunc L x envVal ) t) ann) sigma) *
+      (Heap_okP (p_heap.updatePartFunc H o
+                                       (obj C (p_FM.updatePartFunc FM f (env2fm envVal witn))))
+      ).
+
+    (* 1 *)
+    intros.
+    rename H0 into _1_b.
+    rename X into _1_c.
+
+    (* 2 *)
+    set (L' := (p_env.updatePartFunc L x envVal)).
+    set (FM' := (p_FM.updatePartFunc FM f (env2fm envVal witn))).
+    set (H' := (p_heap.updatePartFunc H o (obj C FM'))).
+    split.
+
+    (* 2b, L z = o_z or L_z = null*)
+    assert ({o_z | envVal = envRef o_z} + (envVal = envNull)) as _2_b.
+    case_eq envVal.
+    intros.
+    apply inr.
+    reflexivity.
+    intros.
+    apply inl.
+    exists r.
+    reflexivity.
+    intros.
+    rewrite H0 in *.
+    inversion _1_c.
+    inversion X.
+    inversion X1.
+
+    (* L z = b(r), show Gamma z must be Box[D] *)
+
+    inversion X0.
+    set (lem := X4 z _ H23).
+    inversion lem.
+    destruct X5.
+    rewrite e0 in H3.
+    simplify_eq H3.
+    destruct s.
+    destruct x2.
+    destruct y1.
+    destruct a.
+    rewrite H26 in H3.
+    simplify_eq H3.
+
+    destruct X5.
+    destruct x2.
+    destruct y1.
+    destruct a.
+    destruct H27.
+    rewrite H23 in H27 .
+    simplify_eq H27.
+
+    rename o into o_y.
+    rename H1 into _2_c.
+    rename H2 into _2_d.
+
+    (* 2 e says that f in fields(C) by reduction rules (this is wrong!)*)
+
+    (* 3 *)
+    inversion _1_c.
+    clear H0 H2 t0 H5 ann0 H6 sigma0 H4 L0 H1.
+    rename X into _3_a.
+    rename X0 into _3_b.
+
+    (* 4 *)
+    inversion _3_a.
+    inversion X.
+    clear y0 H13 f0 H9 x1 H8 eff1 H11 gamma0 H10.
+    unfold typing.subtypeP in *.
+    fold TypeChecksP in *.
+    fold subtypeP in *.
+    unfold typing.fldP in *.
+    fold fldP in *.
+    clear H2 tau.
+
+    clear x0 H4.
+    clear t0 H6.
+    clear H1 eff0.
+    clear e H5.
+    clear gamma H0.
+    rewrite <- H12 in *.
+    clear sigma0 H12.
+    inversion X1.
+    clear eff0 H2 x0 H0 H5 f0 gamma H1.
+    set (_4_a := p_gamma.in_part_func_domain Gamma y (typt_class C1) H4).
+    set (_4_b := p_gamma.in_part_func_domain Gamma z (typt_class C0) H14).
+    rename X1 into _4_c.
+
+    (* unfold subtypeP in H15. *)
+    rename H15 into _4_d.
+    set (Gamma' := p_gamma.updatePartFunc Gamma x (typt_class C0)).
+    fold Gamma' in X0.
+    rename X0 into _4_e.
+
+    clear witn2.
+    rename C0 into D''.
+    rename C into C'.
+    rename C1 into C.
+    rename H6 into _4_f.
+
+    (* 5 *)
+    inversion _3_b.
+    rename H0 into _5_a.
+    rename X0 into _5_b.
+
+    (* 6 *)
+
+    apply (t_frame1 _ _ Gamma' eff).
+    inversion H7.
+    exact H1.
+    exact _4_e.
+    split.
+    exact (subset_preserved _ _ _ _  _  _5_a).
+
+    intros s.
+    case_eq (v_eq_dec s x).
+    intros.
+    clear H0; rewrite -> e in *; clear e s.
+    clear sigma0 H1.
+    assert (p_gamma.func Gamma' x = p_gamma.func Gamma z ) as _6_a.
+    set (lem := proj1 (p_gamma.updatedFuncProp Gamma x (typt_class D'') _) (eq_refl _)).
+    fold Gamma' in lem.
+    transitivity (Some (typt_class D'')).
+    exact lem.
+    symmetry.
+    exact H14.
+
+    assert (p_env.func L' x = p_env.func L z) as _6_b.
+    transitivity (Some envVal).
+    exact (proj1 (p_env.updatedFuncProp L x envVal _) (eq_refl _)).
+    symmetry.
+    exact H3.
+    case_eq _2_b.
+    intros.
+    clear H0 _2_b.
+    destruct s.
+    rewrite -> e in *.
+    rename x0 into o_z.
+    assert (In o_z (p_heap.domain H)).
+    destruct (_5_b z (typt_class D'') H14).
+    destruct s.
+    rewrite e0 in H3.
+    inversion H3.
+    destruct s. destruct x0.
+    destruct y0.
+    destruct a.
+    rewrite H0 in H3.
+    inversion H3.
+    rewrite <- H5 in *.
+    exact x0.
+    destruct s.
+    destruct x0.
+    destruct y0.
+    destruct a.
+    rewrite H0 in H3; inversion H3.
+    set (stays := p_heap.staysInDomain H o_y (obj C' FM') o_z H0).
+    assert (heap_typeof H' o_z stays = heap_typeof H o_z H0) as _6_iv.
+    case_eq (rn_eq_dec o_z o_y).
+    intros.
+    clear H1; rewrite e0 in *.
+    transitivity C'.
+    unfold heap_typeof.
+    assert (p_heap.func H' o_z = Some (obj C' FM')).
+    rewrite e0.
+    unfold H'.
+    exact (proj1 (p_heap.updatedFuncProp H o_y (obj C' FM') _) (eq_refl _)).
+
+    (* TODO: rewrite *)
+    admit.
+    (* rewrite H1. *)
+    (* reflexivity. *)
+    symmetry.
+    unfold heap_typeof.
+
+    (* TODO: rewrite *)
+    admit.
+    (* rewrite e0. *)
+    (* rewrite _2_d. *)
+    (* reflexivity. *)
+    intros.
+    clear H1.
+    set (lem := proj2 (p_heap.updatedFuncProp H o_y (obj C' FM') _) n).
+    fold H' in lem.
+    unfold heap_typeof.
+
+    (* TODO: rewrite *)
+    admit. 
+    (* rewrite lem. *)
+    (* reflexivity. *)
+    unfold WF_Var.
+    apply inl.
+    apply inr.
+    rewrite _6_b.
+    rewrite _6_a.
+    exists (D'', o_z).
+    exists stays.
+    split.
+    exact H3.
+    split.
+    exact H14.
+    rewrite _6_iv.
+    unfold wf_env.subtypeP.
+    (* apply classSub. *)
+    elim (_5_b z (typt_class D'') H14).
+    intro.
+    destruct a.
+    rewrite e0 in H3; inversion H3.
+    destruct s.
+    destruct x0.
+    destruct y0.
+    destruct a.
+    rewrite H1 in H3; inversion H3.
+    rewrite H6 in *.
+    destruct H2.
+    rewrite H14 in H2; inversion H2.
+    rewrite <- H9 in *.
+    rewrite <- H6 in *.
+    (* dependent rewrite H6 in x0. *)
+    assert ((heap_typeof H r x0) = (heap_typeof H o_z H0)).
+    case_eq (p_heap.func H r).
+    intros.
+    destruct b.
+    transitivity c0.
+    unfold heap_typeof.
+
+    (* TODO: rewrite *)
+    admit. 
+    (* rewrite H8. *)
+    (* reflexivity. *)
+    unfold heap_typeof.
+
+    (* TODO: rewrite *)
+    admit. 
+    (* rewrite <- H6. *)
+    (* rewrite H8. *)
+    (* reflexivity. *)
+    intros.
+    elim (proj2 (p_heap.fDomainCompat H r) H8 x0).
+    rewrite <- H8.
+    exact H5.
+    rename _6_iv into _6_d_iv.
+
+    (* 6 e *)
+    intros.
+    destruct b.
+    destruct x0.
+    destruct y0.
+    destruct a.
+    destruct H2.
+    rewrite H14 in H2; discriminate H2.
+
+    (* L z = null *)
+    intros.
+    clear H0.
+    rewrite e in *.
+    apply inl.
+    apply inl.
+    rewrite _6_b.
+    assumption.
+
+
+    (* 7 a *)
+    intros _7 dummy tau _7';    clear dummy.
+    assert (p_gamma.func Gamma' s = p_gamma.func Gamma s) as _7_a.
+    apply (proj2 (p_gamma.updatedFuncProp _ _ _ _) _7).
+    assert (p_env.func L' s = p_env.func L s) as _7_b.
+    apply (proj2 (p_env.updatedFuncProp _ _ _ _) _7).
+    rewrite _7' in _7_a.
+    symmetry in _7_a.
+    set (_7_c := _5_b s tau _7_a).
+
+    case_eq (p_env.func L s).
+    intros.
+    case_eq b.
+    intros.
+    apply inl. apply inl.
+    rewrite H1 in H0.
+    rewrite H0 in _7_b.
+    assumption.
+
+    (* 7 e, b = envRef o_s *)
+    clear _1_c.
+    clear ann.
+    intros.
+    rename r into o_s.
+    rewrite H1 in *.
+    destruct _7_c. (* case analysis on WF-var Gamma L s *)
+    destruct s0.
+    rewrite H0 in e; discriminate e.
+    destruct s0.
+    destruct x0; destruct y0; destruct a; destruct H5.
+    rewrite H2 in H0;    inversion H0.
+    rewrite <- H9 in *; clear H9.
+    clear o_s; rename r into o_s.
+    clear H0 b H1.
+    rename H5 into _7_e_i.
+    rename c into G.
+    rename H6 into _7_e_ii.
+    set (stays := p_heap.staysInDomain H o_y (obj C' FM') o_s x0).
+    fold H' in stays.
+
+    (* 7 e iii *)
+    assert (heap_typeof H o_s x0 = heap_typeof H' o_s stays) as _7_e_iii.
+    case_eq (rn_eq_dec o_s o_y).
+    intros.
+    clear H0. rewrite <- e in *.
+    transitivity C'.
+    unfold heap_typeof.
+
+    (* TODO: rewrite *)
+    admit.
+    (* rewrite _2_d; reflexivity. *)
+    
+    unfold heap_typeof.
+    assert (p_heap.func H' o_y = Some (obj C' FM')).
+    unfold H'.
+    exact (proj1 (p_heap.updatedFuncProp H o_y (obj C' FM') _) (eq_refl _)).
+
+    (* TODO: rewrite *)
+    admit. 
+    (* rewrite e. *)
+    (* rewrite H0. *)
+    (* reflexivity. *)
+    intros.
+    clear H0.
+    
+    set (lem := proj2 (p_heap.updatedFuncProp H o_y (obj C' FM') _) n).
+    fold H' in lem.
+    unfold heap_typeof.
+
+    (* TODO: rewrite *)
+    admit. 
+    (* rewrite lem. *)
+    (* reflexivity. *)
+    (* end 7 e iii *)
+    
+    set (lem := _5_b s tau _7_a).
+    unfold WF_Var.
+    rewrite _7_b.
+    rewrite _7'.
+
+    (* Case analysis L s = null / o / box with H |- Gamma L s
+     * leads to Gamma s = G, typeof(H, o_s) <: G
+     *)
+    destruct lem.
+    destruct s0.
+    apply inl. apply inl. assumption.
+    apply inl.
+    apply inr.
+    destruct s0.
+    destruct x1.
+    exists (c, r).
+    destruct y0.
+    destruct a.
+    rewrite H0 in H2; inversion H2.
+    rewrite H6 in *.
+    assert (In o_s (p_heap.domain H')).
+    assumption.
+    exists H5.
+    split.
+    assumption.
+    split.
+    destruct H1.
+    rewrite H1 in _7_a.
+    symmetry.
+    assumption.
+    assert ((heap_typeof H r x1) = (heap_typeof H' o_s H5)).
+    transitivity (heap_typeof H o_s x0).
+    case_eq (p_heap.func H r).
+    intros.
+    unfold heap_typeof.
+
+    (* TODO: rewrite *)
+    admit. 
+    (* rewrite H8. *)
+    (* rewrite H6 in H8. *)
+    (* rewrite H8. *)
+    (* reflexivity. *)
+    intros.
+    unfold heap_typeof.
+
+    (* TODO: rewrite *)
+    admit. 
+    (* rewrite H8. *)
+    (* rewrite H6 in H8. *)
+    (* rewrite H8. *)
+    (* assumption. *)
+
+    case_eq (rn_eq_dec o_s o_y).
+    intros.
+    clear H8. 
+    transitivity C'.
+    unfold heap_typeof.
+    rewrite e in *.
+
+    (* TODO: rewrite *)
+    admit. 
+    (* rewrite _2_d. reflexivity. *)
+    unfold heap_typeof.
+    assert (p_heap.func H' o_y = Some (obj C' FM')).
+    unfold H'.
+    exact (proj1 (p_heap.updatedFuncProp H o_y (obj C' FM') _) (eq_refl _)).
+
+    (* TODO: rewrite *)
+    admit. 
+    (* rewrite e. *)
+    (* rewrite H8. *)
+    (* reflexivity. *)
+    intros.
+    clear H8.
+    
+    set (lem := proj2 (p_heap.updatedFuncProp H o_y (obj C' FM') _) n).
+    fold H' in lem.
+    unfold heap_typeof.
+
+    (* TODO: rewrite *)
+    admit. 
+    (* rewrite lem. *)
+    (* reflexivity. *)
+    
+    rewrite <- H8.
+    destruct H1.
+    exact H9.
+    
+    destruct s0.
+    destruct x1.
+    destruct y0.
+    destruct a.
+    destruct H1.
+    rewrite H0 in H2; inversion H2.
+
+    destruct s0.
+    destruct x0; destruct y0. destruct a. destruct H5.
+    rewrite H2 in H0; discriminate H0.
+    (* END 7 e!!! *)
+
+    intros.
+    rename r into o_s.
+    rewrite H1 in *.
+
+    (* Case analysis on H |- Gamma ; L ; s to get box prop: *)
+    set (lem := _5_b s tau _7_a).
+    destruct lem.
+    destruct s0.
+    rewrite e in H0; discriminate H0.
+    destruct s0; destruct x0; destruct y0; destruct a.
+    rewrite H2 in H0; discriminate H0.
+    destruct s0; destruct x0; destruct y0; destruct a; destruct H5.
+    rewrite H2 in H0; simplify_eq H0.
+    intro equRef; rewrite equRef in *.
+    clear H0.
+    rewrite _7_a in H5; simplify_eq H5.
+    intro equTy; rewrite equTy in *.
+    rename c into F.
+    rename _7' into _7_f_i_A.
+    assert (In o_s (p_heap.domain H)).
+    rewrite <- equRef.
+    assumption.
+    assert (In o_s (p_heap.domain H')).
+    unfold H'.
+    apply (p_heap.staysInDomain H _ _ o_s).
+    assumption.
+    assert (heap_typeof H o_s H0  = heap_typeof H' o_s H8) as _7_f_ii.
+
+    case_eq (rn_eq_dec o_s o_y).
+    intros.
+    rewrite e in *.
+    clear H9.
+    transitivity C'.
+    unfold heap_typeof.
+
+    (* TODO: rewrite *)
+    admit. 
+    (* rewrite e. *)
+    (* rewrite _2_d. *)
+    (* reflexivity. *)
+
+    
+    unfold heap_typeof.
+    assert (p_heap.func H' o_y = Some (obj C' FM')).
+    apply (p_heap.updatedFuncProp _ _ _ _).
+    reflexivity.
+
+    (* TODO: rewrite *)
+    admit. 
+    (* rewrite e. *)
+    (* rewrite H9. *)
+    (* reflexivity. *)
+    
+    intros.
+    clear H9.
+    case_eq (p_heap.func H o_s).
+    intros.
+    destruct b0.
+    transitivity c.
+    unfold heap_typeof.
+
+    (* TODO: rewrite *)
+    admit.
+    (* rewrite H9. *)
+    (* reflexivity. *)
+
+    
+    assert (p_heap.func H' o_s = Some (obj c f0)).
+    unfold H'.
+    transitivity  (p_heap.func H o_s).
+    apply (proj2 (p_heap.updatedFuncProp H o_y (obj C' FM') o_s) ).
+    assumption.
+    assumption.
+    unfold heap_typeof.
+
+    (* TODO: rewrite *)
+    admit. 
+    (* rewrite H10. *)
+    (* reflexivity. *)
+
+    intros.
+    elim (proj2 (p_heap.fDomainCompat H o_s) H9 H0).
+    unfold WF_Var.
+    rewrite _7_b.
+    rewrite _7_f_i_A.
+    rewrite H2.
+    apply inr.
+    exists (F, o_s).
+    exists H8.
+    split.
+    reflexivity.
+    split.
+    reflexivity.
+    rewrite <- _7_f_ii.
+    assert ((heap_typeof H o_s H0) = (heap_typeof H r x0)
+           ).
+    unfold heap_typeof.
+
+    (* TODO: rewrite *)
+    admit. 
+    (* rewrite equRef. *)
+    (* induction (p_heap.func H o_s); *)
+    (* reflexivity. *)
+    
+    rewrite H9.
+    assumption.
+
+    intro.
+    set (s_in_gamma := p_gamma.in_part_func_domain Gamma s tau _7_a).
+    set (lem := _5_a _ s_in_gamma).
+    elim (proj2 (p_env.fDomainCompat _ _) H0 lem).
+
+    (* HEAP OK *)
+
+    intro.
+    rename o into o_y.
+    rename o0 into o.
+
+    case_eq (rn_eq_dec o_y o).
+    intros; clear H0.
+    rewrite <- e in *.
+    set (lem := proj1 (p_heap.updatedFuncProp H o_y (obj C FM') _) (eq_refl _)).
+    fold H' in lem.
+    rewrite lem in H4.
+    inversion H4.
+    rewrite <- H5 in *.
+    rewrite <- H6 in *.
+    clear H5 H6 C0 FM0.
+    clear lem H4 e o.
+    intro; intros.
+    
+    case_eq (fn_eq_dec f0 f).
+    intros.
+    clear H4; rewrite e in *.
+    set (lem := proj1 (p_FM.updatedFuncProp FM f (env2fm envVal witn) f) (eq_refl _ )).
+    fold FM' in lem.
+    rewrite H0 in lem.
+    inversion lem.
+    induction envVal; 
+    inversion H5.
+    rewrite <- H6 in *.
+    rename o into o_z.
+    rename H3 into _9_b_ii_B.
+    rename H0 into _9_b_ii_A.
+    
+    inversion _1_c.
+    destruct X0.
+    inversion X.
+    inversion X0.
+    set (_9_b_iii_lem := w z (typt_class C0) H23).
+    unfold WF_Var in _9_b_iii_lem.
+    assert ({C_o : class * Ref_type |
+             let (C, o) := C_o in
+             {witn : In o (p_heap.domain H) |
+              p_env.func L z = Some (envRef o) /\
+              p_gamma.func Gamma z = Some (typt_class C) /\
+              wf_env.subtypeP P (typt_class (heap_typeof H o witn))
+                              (typt_class C)}}).
+    induction _9_b_iii_lem.
+    induction a.
+    rewrite a in _9_b_ii_B; simplify_eq _9_b_ii_B.
+    exact b.
+    destruct b; destruct x2; destruct y1; destruct a.
+    rewrite H25 in _9_b_ii_B; simplify_eq _9_b_ii_B.
+    clear _9_b_iii_lem.
+
+    destruct X3; destruct x2; destruct y1; destruct a.
+    rewrite H25 in _9_b_ii_B; simplify_eq _9_b_ii_B.
+    intro ref_eq; rewrite ref_eq in *.
+    destruct H26.
+    rename H26 into _9_b_v_C.
+    rename H27 into _9_b_v_D.
+    rename H25 into _9_b_v_A.
+    assert (In o_z (p_heap.domain H)) as _9_b_v_B.
+    rewrite <- ref_eq; assumption.
+    rewrite _9_b_v_C in H23; simplify_eq H23; intro simpl_eq; rewrite simpl_eq in *.
+    inversion X2.
+
+    set (lemlem := w y (typt_class C1) H28).
+    
+    assert ({C_o : class * Ref_type |
+           let (C, o) := C_o in
+           {witn : In o (p_heap.domain H) |
+           p_env.func L y = Some (envRef o) /\
+           p_gamma.func Gamma y = Some (typt_class C) /\
+           wf_env.subtypeP P (typt_class (heap_typeof H o witn))
+                           (typt_class C)}}).
+    induction lemlem.
+    induction a.
+    rewrite a in H1; simplify_eq H1.
+    assumption.
+
+    destruct b; destruct x4; destruct y1; destruct a; destruct H32.
+    rewrite H32 in H28; simplify_eq H28.
+    destruct X3.
+    destruct x4.
+    destruct y1.
+    destruct a.
+    destruct H32.
+    rewrite H31 in H1; simplify_eq H1; intro equu; rewrite equu in *.
+    rewrite H28 in H32; simplify_eq H32; intro equuu; rewrite <- equuu in *.
+    assert (heap_typeof H r1 x4 = C).
+    unfold heap_typeof.
+
+    (* TODO: rewrite *)
+    admit. 
+    (* rewrite equu. *)
+    (* rewrite H2. *)
+    (* reflexivity. *)
+    
+    rewrite H34 in H33.
+
+    assert ((heap.ftypeP P C f f_witn) = D).
+    rewrite <- H30.
+    symmetry.
+    inversion H33.
+    apply (ftype_subclass _ _ _ _ _ H37).
+    rewrite H35.
+
+    exists (p_heap.staysInDomain H o_y (obj C FM') o_z _9_b_v_B).
+    assert ((heap_typeof H' o_z
+                         (p_heap.staysInDomain H o_y (obj C FM') o_z _9_b_v_B))
+            = (heap_typeof H o_z _9_b_v_B)
+           ).
+    unfold heap_typeof.
+    case_eq (rn_eq_dec o_z o_y).
+    intros.
+
+
+    (* TODO: rewrite *)
+    admit. 
+    (* rewrite e1. *)
+    (* assert (p_heap.func H' o_y = Some (obj C FM')). *)
+    (* apply (p_heap.updatedFuncProp). *)
+    (* reflexivity. *)
+    (* rewrite H37. *)
+    (* rewrite H2. *)
+    (* reflexivity. *)
+    
+    intros.
+    assert (p_heap.func H' o_z = p_heap.func H o_z).
+    apply (p_heap.updatedFuncProp).
+    assumption.
+
+    (* TODO: rewrite *)
+    admit. 
+    (* rewrite H37. *)
+    (* induction (p_heap.func H o_z). *)
+    (* reflexivity. *)
+    Admitted.
+  (*   reflexivity. *)
+  (*   rewrite H36. *)
+
+  (*   assert ((heap_typeof H o_z _9_b_v_B) = (heap_typeof H r0 x2)). *)
+  (*   unfold heap_typeof. *)
+  (*   rewrite ref_eq. *)
+  (*   induction (p_heap.func H o_z). *)
+  (*   reflexivity. *)
+  (*   reflexivity. *)
+  (*   rewrite H37. *)
+  (*   inversion _9_b_v_D. *)
+  (*   apply (subclass_trans P (heap_typeof H r0 x2) C0 D). *)
+  (*   assumption. *)
+  (*   inversion H24. *)
+  (*   assumption. *)
+  (*   inversion witn. *)
+
+  (*   intros. *)
+  (*   clear H4. *)
+
+  (*   assert (p_FM.func FM' f0 = p_FM.func FM f0). *)
+  (*   apply (p_FM.updatedFuncProp). *)
+  (*   assumption. *)
+  (*   rewrite H0 in H4. symmetry in H4. *)
+  (*   set (lem := _1_b o_y C FM H2 f0 o f_witn H4). *)
+  (*   destruct lem. *)
+  (*   exists (p_heap.staysInDomain H o_y (obj C FM') o x0). *)
+
+  (*   assert ((heap_typeof H' o (p_heap.staysInDomain H o_y (obj C FM') o x0)) *)
+  (*           = (heap_typeof H o x0) *)
+  (*          ). *)
+
+  (*   case_eq (rn_eq_dec o o_y). *)
+  (*   intros. *)
+  (*   clear H5. *)
+  (*   unfold heap_typeof. *)
+  (*   rewrite e. *)
+  (*   assert (p_heap.func H' o_y = Some (obj C FM')). *)
+  (*   apply (p_heap.updatedFuncProp). *)
+  (*   reflexivity. *)
+  (*   rewrite H5. *)
+  (*   rewrite H2. *)
+  (*   reflexivity. *)
+  (*   intros . *)
+  (*   unfold heap_typeof. *)
+  (*   assert (p_heap.func H' o = p_heap.func H o). *)
+  (*   apply (p_heap.updatedFuncProp). *)
+  (*   assumption. *)
+  (*   rewrite H6. *)
+  (*   induction (p_heap.func H o); *)
+  (*     reflexivity. *)
+  (*   rewrite H5. *)
+  (*   assumption. *)
+
+  (*   intros. *)
+  (*   assert (p_heap.func H' o = p_heap.func H o). *)
+  (*   apply (p_heap.updatedFuncProp). *)
+  (*   firstorder. *)
+  (*   case_eq (p_heap.func H o). *)
+  (*   intros. *)
+  (*   destruct b. *)
+  (*   rewrite H5 in H4. *)
+  (*   rewrite H6 in H4. *)
+  (*   inversion H4. *)
+  (*   rewrite H8, H9 in *. *)
+  (*   clear H4 H8 H9 c f0. *)
+  (*   intro; intros. *)
+  (*   set (lem := _1_b o C0 FM0 H6 f0 o0 f_witn H4). *)
+  (*   destruct lem. *)
+  (*   exists (p_heap.staysInDomain H o_y (obj C FM') o0 x0). *)
+  (*   assert ((heap_typeof H o0 x0) = (heap_typeof H' o0 (p_heap.staysInDomain H o_y (obj C FM') o0 x0))). *)
+  (*   case_eq (rn_eq_dec o0 o_y). *)
+  (*   intros. *)
+  (*   unfold heap_typeof. *)
+  (*   rewrite e. *)
+  (*   rewrite H2. *)
+  (*   assert (p_heap.func H' o_y = Some (obj C FM')). *)
+  (*   apply (p_heap.updatedFuncProp). *)
+  (*   reflexivity. *)
+  (*   rewrite H8. *)
+  (*   reflexivity. *)
+  (*   intros. *)
+  (*   unfold heap_typeof. *)
+  (*   assert (p_heap.func H o0 = p_heap.func H' o0). *)
+  (*   symmetry. *)
+  (*   apply (p_heap.updatedFuncProp). *)
+  (*   assumption. *)
+  (*   rewrite H8. *)
+  (*   induction (p_heap.func H' o0); *)
+  (*     reflexivity. *)
+  (*   rewrite <- H7. *)
+  (*   assumption. *)
+  (*   intros. *)
+  (*   rewrite H6 in H5. *)
+  (*   rewrite H5 in H4. *)
+  (*   inversion H4. *)
+
+
