reductions.v
@@ -58,18 +58,15 @@ Section Reductions.
   Inductive Reduction_SF :
     sfconfig_type -> sfconfig_type -> Type :=
   | E_Var : forall x y t H L null_ref_box,
-              isTerm t -> 
               p_env.func L y = Some null_ref_box ->
               Reduction_SF ( # H , L , t_let x <- (Var y) t_in t ! )
                         ( # H , (L +++ x --> null_ref_box) , t ! ) 
 
   | E_Null : forall x t H L,
-              isTerm t -> 
-              Reduction_SF ( # H , L , t_let x <- Null t_in t ! )
+               Reduction_SF ( # H , L , t_let x <- Null t_in t ! )
                         ( # H , (L +++ x --> envNull) , t !)
 
   | E_New : forall C o x t H L FM flds,
-              isTerm t ->
               ~ In o (p_heap.domain H) ->
               fieldsP C flds ->
               FM = p_FM.newPartFunc flds FM_null ->
@@ -78,7 +75,6 @@ Section Reductions.
                           ( L +++ x --> envRef o ) , t ! )
 
   | E_Box : forall C o x t H L FM flds,
-              isTerm t ->
               ~ In o (p_heap.domain H) ->
               fieldsP C flds ->
               FM = p_FM.newPartFunc flds FM_null ->
@@ -87,7 +83,6 @@ Section Reductions.
                           ( L +++ x --> envBox o ) , t ! )
 
   | E_Field : forall x y o f t H L C FM fmVal,
-                isTerm t ->
                 p_env.func L y = Some (envRef o) ->
                 p_heap.func H o = Some (obj C FM) ->
                 p_FM.func FM f = Some fmVal ->
@@ -102,7 +97,6 @@ Section Reductions.
    *)
   | E_Assign : forall x y z o f t H L C FM envVal,
                  forall witn: is_not_box envVal, 
-                   isTerm t ->
                    p_env.func L y = Some (envRef o) ->
                    p_heap.func H o = Some (obj C FM) ->
                    In f (p_FM.domain FM) ->
@@ -127,7 +121,7 @@ Section Reductions.
     ann_frame_type.
     destruct F.
     destruct s.
-    exact ( ann_frame (sframe ( e +++ x --> envVal ) e0) a).
+    exact ( ann_frame (sframe ( e +++ x --> envVal ) t) a).
   Defined.
   
   Inductive Reduction_FS : cfg_type -> cfg_type -> Type:=
@@ -139,16 +133,14 @@ Section Reductions.
 
   | E_Return1 : forall H L x y F FS envVal,
                   p_env.func L x = Some envVal ->
-                  Reduction_FS (H, (ann_frame (sframe L (Var x)) (ann_var y)) :: F :: FS)
+                  Reduction_FS (H, (ann_frame (sframe L (TVar x)) (ann_var y)) :: F :: FS)
                                (H, updFrame F y envVal :: FS)
 
   | E_Return2 : forall H L x FS,
-                  Reduction_FS (H, (ann_frame (sframe L (Var x)) ann_epsilon) :: FS)
+                  Reduction_FS (H, (ann_frame (sframe L (TVar x)) ann_epsilon) :: FS)
                                (H, FS)
                                
   | E_Open : forall H L x1 x2 y t1 t2 ann FS o,
-               isTerm t1 ->
-               isTerm t2 ->
                p_env.func L x2 = Some (envBox o) ->
                In o (p_heap.domain H) ->
                Reduction_FS (H, (ann_frame (sframe L
@@ -168,8 +160,6 @@ Section Reductions.
    *)
   | E_Invoke : forall H t' t L L' x y z p m l o C FM FS md Lz,
                  forall (witn: method P C m md), 
-                   isTerm t' ->
-                   isTerm t ->
                    p_env.func L y = Some (envRef o) ->   (* L y = o*)
                    p_env.func L z = Some Lz ->           (* z in dom(L) *)
                    p_heap.func H o = Some (obj C FM) ->  (* H o = <C, FM> *)
