sframe.v
@@ -6,16 +6,6 @@ Require Import namesAndTypes.
 Import ConcreteEverything.
 
 
-Inductive sframe_type := | sframe : Env_type -> ExprOrTerm -> sframe_type.
+Inductive sframe_type := | sframe : Env_type -> Term -> sframe_type.
 Inductive sfconfig_type := | sfconfig :  Heap_type -> sframe_type -> sfconfig_type.
 Notation "( # H , L , t ! )" := (sfconfig H (sframe L t)) (at level 0).
-
-(* Alternatives:
- *  1. Change language to allow exprs, not terms in sframe. Add reduction rules. Modify progress theorem conclusion.
- *
- *  2. Add isTerm here
- *  3. Add isTerm somewhere in well-formedness
- *  4. Don't do anything here, but do not add extra reduction rules. Modify progress theorem conclusion (slightly).
- * 
- *)
-
