typing.v
@@ -17,42 +17,42 @@ Section Typing.
   Definition fldP := fld P.
   Definition ftypeP := ftype P.
 
-  Inductive TypeChecks : Gamma_type -> effect ->
-                         ExprOrTerm -> typecheck_type -> Type :=
+  Inductive TypeChecksExpr : Gamma_type -> effect ->
+                         Expr -> typecheck_type -> Type :=
   | T_Null : forall gamma eff,
-               TypeChecks gamma eff Null typt_all
+               TypeChecksExpr gamma eff Null typt_all
                           
   | T_Var : forall gamma eff x sigma,
               p_gamma.func gamma x = Some sigma ->
-              TypeChecks gamma eff (Var x) sigma
+              TypeChecksExpr gamma eff (Var x) sigma
 
   | T_Field : forall gamma eff x f C,
               forall witn: fldP C f,
                 p_gamma.func gamma x = Some (typt_class C) ->
-                TypeChecks gamma eff (FieldSelection x f)
+                TypeChecksExpr gamma eff (FieldSelection x f)
                            (typt_class (ftypeP C f witn))
 
   | T_Assign : forall gamma eff x f y C D,
                forall witn: fldP C f,
                  p_gamma.func gamma y = Some (typt_class C) ->
-                 TypeChecks gamma eff (FieldSelection x f) (typt_class D) ->
+                 TypeChecksExpr gamma eff (FieldSelection x f) (typt_class D) ->
                  subtypeP (typt_class C) (typt_class D) ->
-                 TypeChecks gamma eff (FieldAssignment x f y) (typt_class C)
+                 TypeChecksExpr gamma eff (FieldAssignment x f y) (typt_class C)
 
   (* TODO: Ocap! *)
   | T_New_ocap :
       forall gamma C,
         ocap P C ->
-        TypeChecks gamma eff_ocap (New C) (typt_class C)
+        TypeChecksExpr gamma eff_ocap (New C) (typt_class C)
 
   | T_New_not_ocap :
       forall gamma C,
-        TypeChecks gamma eff_epsilon (New C) (typt_class C)
+        TypeChecksExpr gamma eff_epsilon (New C) (typt_class C)
 
   | T_Box :
       forall gamma C,
         ocap P C ->
-        TypeChecks gamma eff_ocap (Box C) (typt_box C)
+        TypeChecksExpr gamma eff_ocap (Box C) (typt_box C)
 
 
   | T_Invoke :
@@ -61,24 +61,30 @@ Section Typing.
         p_gamma.func gamma y = Some (typt_class C) ->
         p_gamma.func gamma z = Some sigma ->
         subtypeP sigma (argType md) ->
-        TypeChecks gamma eff (MethodInvocation y m z) (retType md)
+        TypeChecksExpr gamma eff (MethodInvocation y m z) (retType md)
+  
 
   | T_Open : forall gamma eff x C y t sigma,
-               TypeChecks gamma eff (Var x) (typt_box C) ->
-               TypeChecks (p_gamma.updatePartFunc 
+               TypeChecksExpr gamma eff (Var x) (typt_box C) ->
+               TypeChecksTerm (p_gamma.updatePartFunc 
                              p_gamma.emptyPartFunc
                              y (typt_class C)
                           ) eff_ocap t sigma ->
-               TypeChecks gamma eff (Open x y t) (typt_box C)
+               TypeChecksExpr gamma eff (Open x y t) (typt_box C)
+
+  with
+  TypeChecksTerm : Gamma_type -> effect ->
+                   Term -> typecheck_type -> Type :=
 
   | T_Let : forall gamma eff e sigma x tau t,
-              TypeChecks gamma eff e sigma ->
-              TypeChecks (p_gamma.updatePartFunc gamma x sigma) eff
+              TypeChecksExpr gamma eff e sigma ->
+              TypeChecksTerm (p_gamma.updatePartFunc gamma x sigma) eff
                          t tau ->
-              TypeChecks gamma eff (TLet x e t) tau.
+              TypeChecksTerm gamma eff (TLet x e t) tau
 
-  
-  
+  | T_Var_T : forall gamma eff x sigma,
+              p_gamma.func gamma x = Some sigma ->
+              TypeChecksTerm gamma eff (TVar x) sigma.
 
 End Typing.
 
